---
tags:
  - teorema
links:
  - "[[9.2 Derivata]]"
  - "[[9.1 Rapporto incrementale]]"
---
Se $f(a) = f(b) \implies \exists c \in (a,b)$ t.c $f'(c) = \frac{f(b)-f(a)}{b-a}$

##### Dimostrazione
$r(x) = f(a) + \frac{f(b)-f(a)}{b-a} \cdot (x-a)$
$g(x) = f(x) - r(x)$
$g$ Ã¨ continua su $[a,b]$ e derivabile su $(a,b)$
$g(a) = 0$ e $g(b) = 0$, quindi $g(a) = g(b)$, quindi posso applicare il teorema di Rolle a $g$.
$\exists c \in (a,b)$ t.c $g'(c) = 0$
$g'(c) = f'(c) - r'(x)$ = $f'(x) - \frac{f(b)-f(a)}{b-a}$
$g'(c) = 0 \iff f'(c) = \frac{f(b)-f(a)}{b-a}$
